src/vc0/progress.lean
@@ -1,10 +1,192 @@
 import vc0.basic
 
 namespace c0
+open ast
+
+namespace value
+
+theorem default_exists {Γ} (ts) : ∃ (v : value), default Γ ts v :=
+sorry
+
+end value
+
+theorem addr.update.progress {H η R a} :
+  ∃ H' η', addr.update H η R a H' η' :=
+sorry
+
+theorem addr.get.progress {H η a} :
+  ∃ v, addr.get H η a v :=
+sorry
+
+theorem addr.get_len.progress {H η a} :
+  ∃ n, addr.get_len H η a n :=
+sorry
+
+theorem bounds.progress (n : ℕ) (i:int32) :
+  (∃ (j:ℕ), (i:ℤ) = j ∧ j < n) ∨ i < 0 ∨ (n:ℤ) ≤ (i:ℤ) :=
+sorry
+
+theorem alloc_arr.progress (i:int32) :
+  (∃ (j:ℕ), (i:ℤ) = j) ∨ i < 0 :=
+sorry
+
+theorem step_binop.progress {op v₁ v₂} :
+  ∃ v, value.step_binop op v₁ v₂ v :=
+sorry
+
+theorem step_unop.progress {op v} :
+  ∃ v', value.step_unop op v v' :=
+sorry
+
+theorem fdef.progress {Γ : ast} (f : ident) :
+  Γ.is_extern f ∨ Γ.is_fdef f :=
+sorry
+
+theorem step_call.progress {Δ : ctx} {vs} :
+  ∃ η, step_call Δ vs η :=
+sorry
+
+theorem step_ret.progress {Γ E σs H S η τ v}
+  (Sok : stack.ok Γ E σs S τ) (vok : value.ok Γ E v τ) :
+  ∃ s', step_ret ⟨H, S, η⟩ v s' :=
+begin
+  cases Sok,
+  { cases vok, exact ⟨_, step_ret.done⟩ },
+  { exact ⟨_, step_ret.ret⟩ }
+end
+
+theorem step_deref.progress {C a K} :
+  ∃ s', step_deref C a K s' :=
+begin
+  cases a,
+  { exact ⟨_, step_deref.null⟩ },
+  { cases addr.get.progress with v h,
+    exact ⟨_, step_deref.deref h⟩ }
+end
+
+inductive progresses (Γ : ast) (s : state) : Prop
+| final {} : s.final → progresses
+| prog {s'} : step Γ s none s' → progresses
+| io {i} (f : heap × value → state) :
+  (∀ o, step Γ s (some (i, o)) (f o)) → progresses
+open progresses
 
 theorem progress {Γ : ast} (ok : Γ.ok)
-  {s} (h₁ : state.ok Γ s) : s.final ∨ ∃ o s', step Γ s o s' :=
-sorry
+  {s} (stok : state.ok Γ s) : progresses Γ s :=
+begin
+  cases stok,
+  case c0.state.ok.stmt : E σs σ Δ C τ δ s K t Cok tτ sok si Kok {
+    cases Cok with _ _ _ H η S _ _ σok Eok ηok Sok,
+    cases sok,
+    { exact prog (step.decl sok_a) },
+    { exact prog (step.decl_asgn sok_a) },
+    { exact prog step.If₁ },
+    { exact prog step.while },
+    { cases e : lval.is_var sok_lv,
+      { exact prog (step.asgn₁ e) },
+      { exact prog (step.asgn_var₁ e) } },
+    { exact prog step.asnop₁ },
+    { exact prog step.eval₁ },
+    { exact prog step.assert₁ },
+    { cases sok_e,
+      { cases sok_a, cases tτ,
+        cases step_ret.progress Sok value.ok.nil with s' h,
+        exact prog (step.ret_none h) },
+      { exact prog (step.ret₁) } },
+    { cases K,
+      { rcases Kok with ⟨⟨⟩⟩ | Kok,
+        cases Kok.eq_none, cases tτ,
+        cases step_ret.progress Sok value.ok.nil with s' h,
+        exact prog (step.nop₁ h) },
+      { exact prog step.nop₂ } },
+    { exact prog step.seq } },
+  case c0.state.ok.exp : E σs σ H η S Δ ret τ e α K Cok eu lok eok {
+    cases Cok with _ _ _ H η S _ _ σok Eok ηok Sok,
+    rcases eok with ⟨t, eok, tτ⟩,
+    cases α,
+    { cases eok,
+      { exact prog step.int },
+      { exact prog step.bool },
+      { exact prog step.null },
+      { rcases finmap.exists_mem_lookup_iff.2
+          (finmap.mem_keys.1 $ finset.singleton_subset.1 eu) with ⟨τ', iτ'⟩,
+        rcases ηok _ _ iτ' with ⟨v, h, vok⟩,
+        exact prog (step.var h) },
+      { exact prog step.binop₁ },
+      { exact prog step.unop₁ },
+      { exact prog step.cond₁ },
+      { exact prog step.nil },
+      { exact prog step.cons₁ },
+      { exact prog step.call₁ },
+      { exact prog step.field },
+      { exact prog step.deref },
+      { exact prog step.index },
+      { cases value.default_exists _ with v v0,
+        exact prog (step.alloc_ref eok_a v0 ⟨⟩) },
+      { exact prog (step.alloc_arr₁ eok_a) } },
+    { cases lok,
+      { exact prog step.addr_var },
+      { exact prog step.addr_deref₁ },
+      { exact prog step.addr_index₁ },
+      { exact prog step.addr_field₁ } } },
+  case c0.state.ok.ret : E σs σ H η S Δ ret τ α a K Cok aok Kok {
+    cases Cok with _ _ _ H η S _ _ σok Eok ηok Sok,
+    cases Kok,
+    { cases aok,
+      exact prog step.If₂ },
+    { exact prog step.asgn₂ },
+    { cases Kok_a,
+      { exact prog step.asgn_err },
+      { rcases addr.update.progress with ⟨H', η', h⟩,
+        exact prog (step.asgn₃ h) } },
+    { exact prog step.asgn_var₂ },
+    { cases step_deref.progress with s' h,
+      exact prog (step.asnop₂ h) },
+    { exact prog step.eval₂ },
+    { cases aok,
+      exact prog step.assert₂ },
+    { cases step_ret.progress Sok aok with s' h,
+      exact prog (step.ret₂ h) },
+    { cases aok;
+      exact prog step.addr_deref₂ },
+    { cases a,
+      { exact prog step.addr_field_err },
+      { exact prog step.addr_field₂ } },
+    { cases aok;
+      exact prog step.addr_index₂ },
+    { cases aok, cases Kok_a,
+      { exact prog step.addr_index_err₁ },
+      { cases addr.get_len.progress with n h,
+        rcases bounds.progress n aok_1 with ⟨j, h₁, h₂⟩ | h',
+        { exact prog (step.addr_index₃ h h₁ h₂) },
+        { exact prog (step.addr_index_err₂ h h') } } },
+    { exact prog step.binop₂ },
+    { rcases step_binop.progress with ⟨v|err, h⟩,
+      { exact prog (step.binop₃ h) },
+      { exact prog (step.binop_err h) } },
+    { rcases step_unop.progress with ⟨v, h⟩,
+      exact prog (step.unop₂ h) },
+    { cases aok,
+      exact prog step.cond₂ },
+    { exact prog step.cons₂ },
+    { exact prog step.cons₃ },
+    { cases Kok,
+      rcases fdef.progress Kok_f with ext | ⟨τ, Δ, s, h⟩,
+      { exact progresses.io
+          (λ o, state.ret cont_ty.V ⟨o.1, S, η⟩ o.2 Kok_K)
+          (λ ⟨H', v⟩, step.call_extern ext) },
+      { cases step_call.progress with η h',
+        exact prog (step.call₂ h h') } },
+    { cases step_deref.progress with s' h,
+      exact prog (step.deref' h) },
+    { cases aok,
+      rcases alloc_arr.progress aok_1 with ⟨j, h⟩ | h,
+      { cases value.default_exists _ with v v0,
+        exact prog (step.alloc_arr₂ h v0 ⟨⟩) },
+      { exact prog (step.alloc_arr_err h) } } },
+  case c0.state.ok.err : err { exact final state.final.err },
+  case c0.state.ok.done : n { exact final state.final.done },
+end
 
 inductive io_equiv : io → state → io → state → Prop
 | none {s} : io_equiv none s none s
